

The Derivation System *SD*

Shin Kim

`skim@hufs.ac.kr`

교재 3장—진리표—과 4장—진리나무—은 논리 관계의 의미론적 접근 방식을 논의합니다. 한편,

- 교재 5장—*SD* 도출 체계—은 논리 관계의 구조론적 접근 방식을 논의합니다.
 - *SD*는 11가지 도출 법칙으로 구성되며, Fitch diagram을 통해 제시합니다.

Fitch Diagram: An Example

1		$\forall x(Ax \supset Rx)$	
2		$Aa \supset Ra$	$\forall E, 1$
3		Aa	
4		Ra	$\Rightarrow E, 2, 3$
5		$\sim Ra$	
6		$\sim Aa$	$\neg I, 3-5$
7		$\sim La$	
8		$\sim La \supset Aa$	
9		Aa	$\Rightarrow E, 7, 8$
10		$\sim Aa$	$R, 6$
11		La	$\neg E, 7-10$

11 Rules of *SD* by Names

▷ *Reiteration*

11 Rules of *SD* by Names

- ▷ *Reiteration*
- ▷ 5 Introduction Rules:
 $\&I$, $\forall I$, $\sim I$, $\supset I$, $\equiv I$

11 Rules of *SD* by Names

- ▷ *Reiteration*
- ▷ 5 Introduction Rules:
 $\&I, \forall I, \sim I, \supset I, \equiv I$
- ▷ 5 Eliminations Rules:
 $\&E, \forall E, \sim E, \supset E, \equiv E$

11 Rules of *SD* by Requirements

- ▷ The Non-Subderivation Rules¹ of *SD*:
 R , $\&E$, $\&I$, $\vee I$, $\supset E$, $\equiv E$

¹Require No Subderivation

11 Rules of *SD* by Requirements

- ▷ The Non-Subderivation Rules¹ of *SD*:
 $R, \&E, \&I, \vee I, \supset E, \equiv E$
- ▷ The Subderivation Rules² of *SD*:
 $\supset I, \sim I, \sim E, \vee E, \equiv I$

¹Require No Subderivation

²Require Subderivation

Reiteration (R)

1		P
2		P

1		P
2		P

1		A
2		A

Conjunction Elimination (&E)

1		P&Q
2		P

Or,

1		P&Q
2		Q

1		P&Q
2		P

Or,

1		P&Q
2		Q

1		<i>A&B</i>
2		<i>A</i>

Or,

1		<i>A&B</i>
2		<i>B</i>

Conjunction Introduction (&I)

1	P
2	Q
3	P&Q

1	P
2	Q
3	P&Q

1	<i>A</i>
2	<i>B</i>
3	<i>A&B</i>

Disjunction Introduction (\vee I)

1		P
2		P \vee Q

Or,

1		P
2		Q \vee P

$$\begin{array}{l|l} 1 & \mathbf{P} \\ 2 & \mathbf{P} \vee \mathbf{Q} \end{array}$$

Or,

$$\begin{array}{l|l} 1 & \mathbf{P} \\ 2 & \mathbf{Q} \vee \mathbf{P} \end{array}$$

$$\begin{array}{l|l} 1 & A \\ \hline 2 & A \vee B \end{array}$$

Or,

$$\begin{array}{l|l} 1 & A \\ \hline 2 & B \vee A \end{array}$$

Conditional Elimination (\supset E)

1		$\mathbf{P \supset Q}$
2		\mathbf{P}
3		\mathbf{Q}

1		P \supset Q
2		P
3		Q

1		$A \supset B$
2		A
3		B

Biconditional Elimination ($\equiv E$)

1		$P \equiv Q$
2		P
3		Q

Or,

1		$P \equiv Q$
2		Q
3		P

1	$\mathbf{P \equiv Q}$
2	\mathbf{P}
3	\mathbf{Q}

1	$A \equiv B$
2	A
3	B

Or,

1	$\mathbf{P \equiv Q}$
2	\mathbf{Q}
3	\mathbf{P}

Or,

1	$A \equiv B$
2	B
3	A

Conditional Introduction (\supset I)

1		P
2		Q
3		P \supset Q

1		P
2		Q
3		P \supset Q

1		<i>A</i>
2		<i>B</i>
3		<i>A</i> \supset <i>B</i>

Negation Introduction ($\sim I$)

1			P
2			Q
3			\sim Q
4		\sim P	

1		P
2		Q
3		\sim Q
4	\sim P	

1		<i>A</i>
2		<i>B</i>
3		\sim <i>B</i>
4	\sim <i>A</i>	

Negation Elimination (\sim E)

1		$\sim \mathbf{P}$
2		\mathbf{Q}
3		$\sim \mathbf{Q}$
4	\mathbf{P}	

1		$\sim \mathbf{P}$
2		\mathbf{Q}
3		$\sim \mathbf{Q}$
4	\mathbf{P}	

1		$\sim A$
2		B
3		$\sim B$
4	A	

Disjunction Elimination ($\vee E$)

1	$P \vee Q$
2	P
3	R
4	Q
5	R
6	R

1		P \vee Q
2		P
3		R
4		Q
5		R
6		R

1		$A \vee B$
2		A
3		C
4		B
5		C
6		C

Biconditional Introduction ($\equiv I$)

1		P
		—
2		Q
		—
3		Q
		—
4		P
5		P \equiv Q

1		P
		—
2		Q
		—
3		Q
		—
4		P
		—
5		P \equiv Q

1		<i>A</i>
		—
2		<i>B</i>
		—
3		<i>B</i>
		—
4		<i>A</i>
		—
5		<i>A</i> \equiv <i>B</i>